src/program_proof/simplepb/apps/byte_map_proof.v
@@ -1,0 +1,84 @@
+From Perennial.program_proof Require Import grove_prelude.
+From Perennial.goose_lang.lib Require Import typed_map map.impl.
+
+Section proof.
+
+Context `{!heapGS Σ}.
+Definition own_byte_map (mptr:loc) (m:gmap u64 (list u8)): iProp Σ :=
+  ∃ (kvs_sl:gmap u64 Slice.t),
+    "Hkvs_map" ∷ is_map mptr 1 kvs_sl ∗
+    "#Hkvs_slices" ∷ (∀ (k:u64), readonly (is_slice_small (default Slice.nil (kvs_sl !! k))
+                                                          byteT
+                                                          1
+                                                          (default [] (m !! k))
+                                                          )
+                     )
+.
+
+Lemma wp_byteMapGet mptr m (k:u64) :
+  {{{ own_byte_map mptr m }}}
+    Fst (MapGet #mptr #k)
+  {{{
+        sl, RET (slice_val sl);
+        readonly (is_slice_small sl byteT 1 (default [] (m !! k))) ∗
+        own_byte_map mptr m
+  }}}
+.
+Proof.
+  iIntros (Φ) "Hmap HΦ".
+  iNamed "Hmap".
+  wp_apply (wp_MapGet with "Hkvs_map").
+  iIntros (sl ok) "[%Hlookup Hkvs_map]".
+  wp_pures.
+  iApply "HΦ".
+  iSplitR "Hkvs_map"; last first.
+  { iExists _. eauto with iFrame. }
+  iModIntro.
+  iSpecialize ("Hkvs_slices" $! k).
+  rewrite /map_get in Hlookup.
+  apply (f_equal fst) in Hlookup.
+  simpl in Hlookup.
+  rewrite Hlookup.
+  iFrame "#".
+Qed.
+
+Lemma wp_byteMapPut mptr m (k:u64) sl (v:list u8) q :
+{{{
+      own_byte_map mptr m ∗ is_slice_small sl byteT q v
+}}}
+    MapInsert #mptr #k (slice_val sl)
+{{{
+      RET #(); own_byte_map mptr (<[k := v]> m)
+}}}
+.
+Proof.
+  iIntros (Φ) "[Hmap Hsl] HΦ".
+  iNamed "Hmap".
+  iMod (readonly_alloc (is_slice_small sl byteT 1 v) with "[Hsl]") as "#Hsl".
+  { done. }
+  wp_apply (wp_MapInsert with "Hkvs_map").
+  { done. }
+  iIntros "Hkvs_map".
+  iApply "HΦ".
+  iExists _.
+  iFrame "Hkvs_map".
+  rewrite /typed_map.map_insert.
+  iIntros (?).
+  destruct (decide (k0 = k)).
+  {
+    rewrite e.
+    repeat rewrite lookup_insert.
+    simpl.
+    done.
+  }
+  {
+    rewrite lookup_insert_ne; last done.
+    rewrite lookup_insert_ne; last done.
+    iApply "Hkvs_slices".
+  }
+Qed.
+
+Definition has_byte_map_encoding (enc:list u8) (m:gmap u64 (list u8)) : Prop.
+Admitted.
+
+End proof.
